Rustabelle.thy
@@ -8,7 +8,7 @@ type_synonym ('state, 'ans) sem = "('state, 'ans) cont \<Rightarrow> ('state, 'a
 abbreviation seq :: "('state, 'ans) sem \<Rightarrow> ('state, 'ans) sem \<Rightarrow> ('state, 'ans) sem" (infixl ";" 80) where
   "seq s1 s2 \<equiv> s1 \<circ> s2"
 
-definition loop :: "('state \<Rightarrow> 'state \<times> ('state, 'ans) cont option) \<Rightarrow> 'state \<Rightarrow> 'ans" where
+(*definition loop :: "('state \<Rightarrow> 'state \<times> ('state, 'ans) cont option) \<Rightarrow> 'state \<Rightarrow> 'ans" where
   "loop l s = (let (s,s',c) = while (\<lambda>(s,s',c). c = None) (\<lambda>(s,s',c). (s',(l s'))) (s,(l s)) in the c s')"
 
 lemma loop_rule:
@@ -35,7 +35,18 @@ proof-
   term "{((s\<^sub>1,s\<^sub>1',c\<^sub>1), (s\<^sub>2,s\<^sub>2',c\<^sub>2)) | s\<^sub>1 s\<^sub>1' c\<^sub>1 s\<^sub>2 s\<^sub>2' c\<^sub>2. (s\<^sub>1,s\<^sub>2) \<in> r}"
   apply (rule while_rule[where P="\<lambda>(s,s',c). P s \<and> (s',c) = l s" and r=?r'])
   apply (auto simp: assms)[3]
-  apply (rule assms(4))
+  apply (rule assms(4))*)
+
+definition loop :: "('state \<Rightarrow> 'state \<times> bool) \<Rightarrow> 'state \<Rightarrow> 'state" where
+  "loop l s = (let (s,s',c) = while (\<lambda>(s,s',c). c) (\<lambda>(s,s',c). (s',(l s'))) (s,(l s)) in s')"
+
+lemma loop_rule:
+  assumes "P s"
+  assumes "\<And>s s'. P s \<Longrightarrow> l s = (s',True) \<Longrightarrow> P s'" "\<And>s s' c. P s \<Longrightarrow> l s = (s',False) \<Longrightarrow> Q s'"
+  assumes "wf r" "\<And>s s'. P s \<Longrightarrow> l s = (s',True) \<Longrightarrow> (s', s) \<in> r"
+  shows "Q (loop l s)"
+sorry
+
 
 type_synonym u32 = nat
 
