Export.thy
@@ -28,17 +28,17 @@ type_synonym state = "nat \<rightharpoonup> Any"
 
 
 
-definition fac_16 where "fac_16 cont_27 s = ((\<lambda>cont s. cont (s(12 \<mapsto> Any_12 core_iter_ops_Range_A__Iterator_next)));
+definition fac_16 where "fac_16 s = ((\<lambda>cont s. cont (s(12 \<mapsto> Any_12 core_iter_ops_Range_A__Iterator_next)));
 (\<lambda>cont s. cont (s(14 \<mapsto> Any_14 (case s 3 of Some (Any_3 x) => x))));
 (\<lambda>cont s. cont (s(13 \<mapsto> Any_13 (case s 14 of Some (Any_14 x) => x))));
 (\<lambda>cont s. cont (let (t11, t13) = ((case s 12 of Some (Any_12 x) => x) (case s 13 of Some (Any_13 x) => x)) in s(11 \<mapsto> Any_11 t11, 13 \<mapsto> Any_13 t13)));
-(\<lambda>cont s. case (case s 11 of Some (Any_11 x) => x) of core_option_Option_None  => (cont_27) cont s | core_option_Option_Some _ => ((\<lambda>cont s. cont (s(4 \<mapsto> Any_4 (case (case s 11 of Some (Any_11 x) => x) of core_option_Option_Some x => x))));
+(\<lambda>cont s. case (case s 11 of Some (Any_11 x) => x) of core_option_Option_None  => ((\<lambda>cont s. (s,False))) cont s | core_option_Option_Some _ => ((\<lambda>cont s. cont (s(4 \<mapsto> Any_4 (case (case s 11 of Some (Any_11 x) => x) of core_option_Option_Some x => x))));
 (\<lambda>cont s. cont (s(16 \<mapsto> Any_16 (case s 4 of Some (Any_4 x) => x))));
 (\<lambda>cont s. cont (s(1 \<mapsto> Any_1 ((case s 1 of Some (Any_1 x) => x) * (case s 16 of Some (Any_16 x) => x)))));
 (\<lambda>cont s. cont (s(15 := None)));
 (\<lambda>cont s. cont (s(13 := None)));
 (\<lambda>cont s. cont (s(14 := None)));
-id) cont s)) (\<lambda>s. (s, None)) s"
+id) cont s)) (\<lambda>s. (s, True)) s"
 
 definition fac :: "u32 => u32" where
 "fac n = ((\<lambda>cont s. cont (s(0 \<mapsto> Any_0 n)));
@@ -48,7 +48,7 @@ definition fac :: "u32 => u32" where
 (\<lambda>cont s. cont (s(9 \<mapsto> Any_9 (core_ops_Range 2 (case s 10 of Some (Any_10 x) => x)))));
 (\<lambda>cont s. cont (let (t7) = ((case s 8 of Some (Any_8 x) => x) (case s 9 of Some (Any_9 x) => x)) in s(7 \<mapsto> Any_7 t7)));
 (\<lambda>cont s. cont (s(3 \<mapsto> Any_3 (case s 7 of Some (Any_7 x) => x))));
-(\<lambda>cont. loop (fac_16 ((\<lambda>cont s. cont (s(13 := None)));
+(\<lambda>cont s. cont (loop fac_16 s)); (\<lambda>cont s. cont (s(13 := None)));
 (\<lambda>cont s. cont (s(14 := None)));
 (\<lambda>cont s. cont (s(3 := None)));
 (\<lambda>cont s. cont (s(7 := None)));
@@ -58,6 +58,6 @@ definition fac :: "u32 => u32" where
 (\<lambda>cont s. cont (s(6 := None)));
 (\<lambda>cont s. cont (s(18 \<mapsto> Any_18 (case s 1 of Some (Any_1 x) => x))));
 (\<lambda>cont s. cont (s(19 \<mapsto> Any_19 (case s 18 of Some (Any_18 x) => x))));
-id)))) (\<lambda>s. (case s 19 of Some (Any_19 x) => x)) Map.empty"
+id::(state,u32) sem) (\<lambda>s. (case s 19 of Some (Any_19 x) => x)) Map.empty"
 
 end
